First implementation of leadsto; sorrys arising from locale imprecisions missing

Worklist_Algorithms/Liveness_Subsumption_Impl.thy
@@ -14,15 +14,15 @@ locale Liveness_Search_Space_Key_Impl_Defs =
 locale Liveness_Search_Space_Key_Impl =
   Liveness_Search_Space_Key_Impl_Defs +
   Liveness_Search_Space_Key +
-  assumes [sepref_fr_rules]: "(uncurry0 a\<^sub>0i, uncurry0 (RETURN (PR_CONST a\<^sub>0))) \<in> unit_assn\<^sup>k \<rightarrow>\<^sub>a A"
-  assumes [sepref_fr_rules]: "(Fi,RETURN o PR_CONST F') \<in> A\<^sup>k \<rightarrow>\<^sub>a bool_assn"
-  assumes [sepref_fr_rules]: "(uncurry Lei,uncurry (RETURN oo PR_CONST op \<preceq>)) \<in> A\<^sup>k *\<^sub>a A\<^sup>k \<rightarrow>\<^sub>a bool_assn"
-  assumes [sepref_fr_rules]: "(succsi,RETURN o PR_CONST succs) \<in> A\<^sup>k \<rightarrow>\<^sub>a list_assn A"
-  assumes [sepref_fr_rules]: "(keyi,RETURN o PR_CONST key) \<in> A\<^sup>k \<rightarrow>\<^sub>a id_assn"
-  assumes [sepref_fr_rules]: "(copyi, RETURN o COPY) \<in> A\<^sup>k \<rightarrow>\<^sub>a A"
+  assumes refinements[sepref_fr_rules]:
+    "(uncurry0 a\<^sub>0i, uncurry0 (RETURN (PR_CONST a\<^sub>0))) \<in> unit_assn\<^sup>k \<rightarrow>\<^sub>a A"
+    "(Fi,RETURN o PR_CONST F') \<in> A\<^sup>k \<rightarrow>\<^sub>a bool_assn"
+    "(uncurry Lei,uncurry (RETURN oo PR_CONST op \<preceq>)) \<in> A\<^sup>k *\<^sub>a A\<^sup>k \<rightarrow>\<^sub>a bool_assn"
+    "(succsi,RETURN o PR_CONST succs) \<in> A\<^sup>k \<rightarrow>\<^sub>a list_assn A"
+    "(keyi,RETURN o PR_CONST key) \<in> A\<^sup>k \<rightarrow>\<^sub>a id_assn"
+    "(copyi, RETURN o COPY) \<in> A\<^sup>k \<rightarrow>\<^sub>a A"
 
-
-context Liveness_Search_Space_Key_Impl_Defs
+context Liveness_Search_Space_Key_Defs
 begin
 
 (* XXX The lemma has this form to avoid unwanted eta-expansions.
@@ -101,7 +101,7 @@ lemmas alt_defs =
   check_subsumption_map_list_extract pop_map_list_alt_def push_map_list_alt_def
 
 lemma dfs_map_alt_def:
-  "dfs_map P = do {
+  "dfs_map = (\<lambda> P. do {
     (P,ST,r) \<leftarrow> RECT (\<lambda>dfs (P,ST,v).
       let (ST, b) = (ST, check_subsumption_map_list v ST) in
       if b then RETURN (P, ST, True)
@@ -120,11 +120,38 @@ lemma dfs_map_alt_def:
       }
     ) (P,Map.empty,a\<^sub>0);
     RETURN (r, P)
-  }"
+  })"
   unfolding dfs_map_def
   unfolding Let_def
   unfolding COPY_def
   by auto
+
+definition dfs_map' where
+  "dfs_map' a P \<equiv> do {
+    (P,ST,r) \<leftarrow> RECT (\<lambda>dfs (P,ST,v).
+      let (ST, b) = (ST, check_subsumption_map_list v ST) in
+      if b then RETURN (P, ST, True)
+      else do {
+        let (P, b1) = (P, check_subsumption_map_set v P) in
+        if b1 then
+          RETURN (P, ST, False)
+        else do {
+            let (_, ST1) = (None :: 'v option, push_map_list (COPY v) ST);
+            (P1, ST2, r) \<leftarrow>
+              nfoldli (succs v) (\<lambda>(_,_,b). \<not>b) (\<lambda>v' (P,ST,_). dfs (P,ST,v')) (P,ST1,False);
+            let (_, ST') = (None :: 'v option, pop_map_list (COPY v) ST2);
+            let (_, P') = (None :: 'v option, insert_map_set (COPY v) P1);
+            RETURN (P', ST', r)
+          }
+      }
+    ) (P,Map.empty,a);
+    RETURN (r, P)
+  }"
+
+lemma dfs_map'_id:
+  "dfs_map' a\<^sub>0 = dfs_map"
+  apply (subst dfs_map_alt_def)
+  unfolding dfs_map'_def ..
 
 end (* Search Space Nodes Empty Key Impl Defs 1 *)
 
@@ -182,16 +209,46 @@ lemma [def_pat_rules]:
   "keyi \<equiv> UNPROTECT keyi" "key \<equiv> UNPROTECT key"
   by simp_all
 
-(* lemma [safe_constraint_rules]: "CN_FALSE is_pure A \<Longrightarrow> is_pure A" by simp *)
+abbreviation "passed_assn \<equiv> hm.hms_assn' id_assn (lso_assn A)"
 
-sepref_thm dfs_map1_impl is
-  "uncurry0 (do {(r, p) \<leftarrow> dfs_map Map.empty; RETURN r})" :: "unit_assn\<^sup>k \<rightarrow>\<^sub>a bool_assn"
+(* This is to make the pre-processing phase pick the right type for the input *)
+lemma [intf_of_assn]:
+  "intf_of_assn (hm.hms_assn' a b) TYPE(('aa, 'bb) i_map)"
+  by simp
+
+sepref_definition dfs_map_impl is
+  "PR_CONST dfs_map" :: "passed_assn\<^sup>d \<rightarrow>\<^sub>a prod_assn bool_assn passed_assn"
+  unfolding PR_CONST_def
   apply (subst dfs_map_alt_def)
   unfolding alt_defs
   unfolding Bex_set list_ex_foldli
   unfolding fold_lso_bex
   unfolding lso_fold_custom_empty hm.hms_fold_custom_empty HOL_list.fold_custom_empty
-  supply [[goals_limit = 1]]
+  by sepref
+
+sepref_register dfs_map
+
+lemmas [sepref_fr_rules] = dfs_map_impl.refine_raw
+
+lemma passed_empty_refine[sepref_fr_rules]:
+  "(uncurry0 hm.hms_empty, uncurry0 (RETURN (PR_CONST hm.op_hms_empty))) \<in> unit_assn\<^sup>k \<rightarrow>\<^sub>a passed_assn"
+  by (rule hfrefI, auto simp: pure_unit_rel_eq_empty intro!: sepref_fr_rules(14)[simplified])
+
+sepref_register hm.op_hms_empty
+
+sepref_thm dfs_map_impl' is
+  "uncurry0 (do {(r, p) \<leftarrow> dfs_map Map.empty; RETURN r})" :: "unit_assn\<^sup>k \<rightarrow>\<^sub>a bool_assn"
+  unfolding hm.hms_fold_custom_empty by sepref
+
+sepref_definition dfs_map'_impl is
+  "uncurry dfs_map'"
+  :: "A\<^sup>d *\<^sub>a (hm.hms_assn' id_assn (lso_assn A))\<^sup>d \<rightarrow>\<^sub>a bool_assn \<times>\<^sub>a hm.hms_assn' id_assn (lso_assn A)"
+  unfolding dfs_map'_def
+  unfolding PR_CONST_def
+  unfolding alt_defs
+  unfolding Bex_set list_ex_foldli
+  unfolding fold_lso_bex
+  unfolding lso_fold_custom_empty hm.hms_fold_custom_empty HOL_list.fold_custom_empty
   by sepref
 
 end (* Search Space Nodes Finite Strict Key Impl 1 *)
