Worklist_Algorithms/Leadsto_Impl.thy
@@ -1,0 +1,92 @@
+theory Leadsto_Impl
+  imports Leadsto_Map Unified_PW_Impl Liveness_Subsumption_Impl
+begin
+
+(* XXX Move *)
+definition
+  "list_of_set S = SPEC (\<lambda>l. set l = S)"
+
+(* XXX Move *)
+lemma lso_id_hnr:
+  "(return o id, list_of_set) \<in> (lso_assn A)\<^sup>d \<rightarrow>\<^sub>a list_assn A"
+  unfolding list_of_set_def lso_assn_def hr_comp_def br_def by sepref_to_hoare sep_auto
+
+sepref_register hm.op_hms_empty
+
+context Worklist_Map2_Impl
+begin
+
+sepref_thm pw_algo_map2_impl is
+  "uncurry0 (pw_algo_map2)" ::
+  "unit_assn\<^sup>k \<rightarrow>\<^sub>a bool_assn \<times>\<^sub>a (hm.hms_assn' id_assn (lso_assn A))"
+  unfolding pw_algo_map2_def add_pw'_map2_alt_def PR_CONST_def
+  supply [[goals_limit = 1]]
+  supply conv_to_is_Nil[simp]
+  unfolding fold_lso_bex
+  unfolding take_from_list_alt_def
+  apply (rewrite in "{a\<^sub>0}" lso_fold_custom_empty)
+  unfolding hm.hms_fold_custom_empty
+  apply (rewrite in "[a\<^sub>0]" HOL_list.fold_custom_empty)
+   apply (rewrite in "{}" lso_fold_custom_empty)
+  unfolding F_split (* XXX Why? F only appears in the invariant *)
+  by sepref
+
+concrete_definition (in -) pw_impl
+for Lei a\<^sub>0i Fi succsi emptyi
+uses Worklist_Map2_Impl.pw_algo_map2_impl.refine_raw is "(uncurry0 ?f,_)\<in>_"
+
+end (* Worklist Map 2 Impl *)
+
+locale Leadsto_Search_Space_Key_Impl =
+  Leadsto_Search_Space_Key a\<^sub>0 F _ empty _ E key F' _ _ P Q succs succs1 +
+  Liveness_Search_Space_Key_Impl a\<^sub>0 F _ V empty succs E key A succsi a\<^sub>0i Lei keyi copyi
+  for key :: "'v :: {heap} \<Rightarrow> 'k :: {hashable,heap}"
+  and a\<^sub>0 F F' copyi P Q V empty succs succs1 E A succsi a\<^sub>0i Lei keyi +
+  fixes succs1i and Lei' and Pi Qi
+  assumes  succs1_impl: "(succs1i, (RETURN \<circ>\<circ> PR_CONST) succs1) \<in> A\<^sup>k \<rightarrow>\<^sub>a list_assn A"
+    and Lei': "(uncurry Lei', uncurry ((RETURN \<circ>\<circ>\<circ> PR_CONST) op \<unlhd>)) \<in> A\<^sup>k *\<^sub>a A\<^sup>k \<rightarrow>\<^sub>a bool_assn"
+    and [sepref_fr_rules]: "(Pi,RETURN o P) \<in> A\<^sup>k \<rightarrow>\<^sub>a bool_assn" "(Qi,RETURN o Q) \<in> A\<^sup>k \<rightarrow>\<^sub>a bool_assn"
+begin
+
+sublocale Worklist_Map2_Impl _ _ "\<lambda> _. False" _ succs1 _ _ "(\<lambda>_. False)" _ succs1i _ _ Lei'
+  by (standard; rule refinements Lei' succs1_impl)
+
+sepref_register pw_algo_map2_copy
+sepref_register P Q
+
+lemmas [sepref_fr_rules] = lso_id_hnr ran_of_map_impl.refine[folded hm.hms_assn'_id_hms_assn]
+
+lemma pw_algo_map2_copy_fold:
+  "PR_CONST pw_algo_map2_copy = A'.pw_algo_map2"
+  unfolding pw_algo_map2_copy_def by simp
+
+lemmas [sepref_fr_rules] = pw_algo_map2_impl.refine_raw[folded pw_algo_map2_copy_fold]
+
+definition "has_cycle_map_copy \<equiv> has_cycle_map"
+
+lemma has_cycle_map_copy_fold:
+  "PR_CONST has_cycle_map_copy = has_cycle_map"
+  unfolding has_cycle_map_copy_def by simp
+
+sepref_register has_cycle_map_copy
+
+lemma has_cycle_map_fold:
+  "has_cycle_map = dfs_map'"
+  unfolding has_cycle_map_def dfs_map'_def
+  by (subst Liveness_Search_Space_Key_Defs.dfs_map_alt_def) standard
+
+lemmas [sepref_fr_rules] =
+  dfs_map'_impl.refine_raw[folded has_cycle_map_fold, folded has_cycle_map_copy_fold]
+
+sepref_definition leadsto_impl is
+  "uncurry0 leadsto_map4'" :: "unit_assn\<^sup>k \<rightarrow>\<^sub>a bool_assn"
+  unfolding leadsto_map4'_def
+  unfolding pw_algo_map2_copy_def[symmetric]
+  unfolding has_cycle_map_copy_def[symmetric]
+  unfolding hm.hms_fold_custom_empty
+  unfolding list_of_set_def[symmetric]
+  by sepref
+
+end (* Leadsto Search Space Key Impl *)
+
+end (* End of theory *)
