Worklist_Algorithms/Leadsto_Map.thy
@@ -1,0 +1,742 @@
+theory Leadsto_Map
+  imports Leadsto Unified_PW_Hashing Liveness_Subsumption_Map Heap_Hash_Map Next_Key
+begin
+
+definition map_to_set :: "('b \<rightharpoonup> 'a set) \<Rightarrow> 'a set" where
+  "map_to_set m = (\<Union> (ran m))"
+
+hide_const wait
+
+definition
+  "map_list_set_rel =
+    {(ml, ms). dom ml = dom ms
+     \<and> (\<forall> k \<in> dom ms. set (the (ml k)) = the (ms k) \<and> distinct (the (ml k)))
+     \<and> finite (dom ml)
+    }"
+
+context Worklist_Map2_Defs
+begin
+
+definition
+  "add_pw'_map3 passed wait a \<equiv>
+   nfoldli (succs a) (\<lambda>(_, _, brk). \<not>brk)
+    (\<lambda>a (passed, wait, _).
+      do {
+      (* ASSERT (\<forall> wait \<in> ran wait. \<forall> x \<in> set wait. \<not> empty x); *)
+      RETURN (
+        if empty a then
+            (passed, wait, False)
+        else if F' a then (passed, wait, True)
+        else
+          let k = key a; passed' = (case passed k of Some passed' \<Rightarrow> passed' | None \<Rightarrow> [])
+          in
+            if \<exists> x \<in> set passed'. a \<unlhd> x then
+              (passed, wait, False)
+            else
+              (passed(k \<mapsto> (a # passed')), a # wait, False)
+        )
+      }
+    )
+    (passed,wait,False)"
+
+definition
+  "pw_map_inv3 \<equiv> \<lambda> (passed, wait, brk).
+    \<exists> passed'. (passed, passed') \<in> map_list_set_rel \<and> pw_map_inv (passed', wait, brk)
+  "
+
+definition pw_algo_map3 where
+  "pw_algo_map3 = do
+    {
+      if F a\<^sub>0 then RETURN (True, Map.empty)
+      else if empty a\<^sub>0 then RETURN (False, Map.empty)
+      else do {
+        (passed, wait) \<leftarrow> RETURN ([key a\<^sub>0 \<mapsto> [a\<^sub>0]], [a\<^sub>0]);
+        (passed, wait, brk) \<leftarrow> WHILEIT pw_map_inv3 (\<lambda> (passed, wait, brk). \<not> brk \<and> wait \<noteq> [])
+          (\<lambda> (passed, wait, brk). do
+            {
+              (a, wait) \<leftarrow> take_from_list wait;
+              ASSERT (reachable a);
+              if empty a then RETURN (passed, wait, brk) else add_pw'_map3 passed wait a
+            }
+          )
+          (passed, wait, False);
+          RETURN (brk, passed)
+      }
+    }
+  "
+
+end -- \<open>Worklist Map 2 Defs\<close>
+
+lemma map_list_set_rel_empty[refine, simp, intro]:
+  "(Map.empty, Map.empty) \<in> map_list_set_rel"
+  unfolding map_list_set_rel_def by auto
+
+lemma map_list_set_rel_single:
+  "(ml(key a\<^sub>0 \<mapsto> [a\<^sub>0]), ms(key a\<^sub>0 \<mapsto> {a\<^sub>0})) \<in> map_list_set_rel" if "(ml, ms) \<in> map_list_set_rel"
+  using that unfolding map_list_set_rel_def by auto
+
+context Worklist_Map2
+begin
+
+lemma refine_start[refine]:
+  "(([key a\<^sub>0 \<mapsto> [a\<^sub>0]], [a\<^sub>0]), [key a\<^sub>0 \<mapsto> {a\<^sub>0}], [a\<^sub>0]) \<in> map_list_set_rel \<times>\<^sub>r Id"
+  by (simp add: map_list_set_rel_single)
+
+lemma pw_map_inv_ref:
+  "pw_map_inv (x1, x2, x3) \<Longrightarrow> (x1a, x1) \<in> map_list_set_rel \<Longrightarrow> pw_map_inv3 (x1a, x2, x3)"
+  unfolding pw_map_inv3_def by auto
+
+lemma refine_aux[refine]:
+  "(x1, x) \<in> map_list_set_rel \<Longrightarrow> ((x1, x2, False), x, x2, False) \<in> map_list_set_rel \<times>\<^sub>r Id \<times>\<^sub>r Id"
+  by simp
+
+lemma map_list_set_relD:
+  "ms k = Some (set xs)" if "(ml, ms) \<in> map_list_set_rel" "ml k = Some xs"
+  using that unfolding map_list_set_rel_def
+  by clarsimp (metis (mono_tags, lifting) domD domI option.sel)
+
+lemma map_list_set_rel_distinct:
+  "distinct xs" if "(ml, ms) \<in> map_list_set_rel" "ml k = Some xs"
+  using that unfolding map_list_set_rel_def by clarsimp (metis domI option.sel)
+
+lemma map_list_set_rel_NoneD1[dest, intro]:
+  "ms k = None" if "(ml, ms) \<in> map_list_set_rel" "ml k = None"
+  using that unfolding map_list_set_rel_def by auto
+
+lemma map_list_set_rel_NoneD2[dest, intro]:
+  "ml k = None" if "(ml, ms) \<in> map_list_set_rel" "ms k = None"
+  using that unfolding map_list_set_rel_def by auto
+
+lemma map_list_set_rel_insert:
+  "(ml, ms) \<in> map_list_set_rel \<Longrightarrow>
+   ml (key a) = Some xs \<Longrightarrow>
+   ms (key a) = Some (set xs) \<Longrightarrow>
+   a \<notin> set xs \<Longrightarrow>
+   (ml(key a \<mapsto> a # xs), ms(key a \<mapsto> insert a (set xs))) \<in> map_list_set_rel"
+  apply (frule map_list_set_rel_distinct) unfolding map_list_set_rel_def by auto
+
+lemma add_pw'_map3_ref:
+  "add_pw'_map3 ml xs a \<le> \<Down> (map_list_set_rel \<times>\<^sub>r Id) (add_pw'_map2 ms xs a)"
+  if "(ml, ms) \<in> map_list_set_rel" "\<not> empty a"
+  using that unfolding add_pw'_map3_def add_pw'_map2_def
+  apply refine_rcg
+     apply refine_dref_type
+     apply (simp; fail)
+    apply (simp; fail)
+   apply (simp; fail)
+  apply (clarsimp simp: Let_def)
+  apply safe
+  subgoal
+    by (auto dest: map_list_set_relD[OF _ sym])
+  subgoal
+    apply (auto split: option.split_asm)
+    by (metis (mono_tags, lifting)
+          map_list_set_relD map_list_set_rel_NoneD1 option.collapse option.sel option.simps(3)
+        )
+  subgoal premises prems for a ms x2a ml x2c
+  proof (cases "ml (key a)")
+    case None
+    with \<open>(ml, ms) \<in> map_list_set_rel\<close> have "ms (key a) = None"
+      by auto
+    with None \<open>(ml, ms) \<in> map_list_set_rel\<close> show ?thesis
+      by (auto intro: map_list_set_rel_single)
+  next
+    case (Some xs)
+    from map_list_set_relD[OF \<open>(ml, ms) \<in> map_list_set_rel\<close> \<open>ml _ = _\<close>] have
+      "ms (key a) = Some (set xs)"
+      by auto
+    moreover from prems have "a \<notin> set xs"
+      by (metis Some empty_subsumes' local.eq_refl)
+    ultimately show ?thesis
+      using Some \<open>(ml, ms) \<in> map_list_set_rel\<close> by (auto intro: map_list_set_rel_insert)
+  qed
+  done
+
+lemma pw_algo_map3_ref[refine]:
+  "pw_algo_map3 \<le> \<Down> (Id \<times>\<^sub>r map_list_set_rel) pw_algo_map2"
+  unfolding pw_algo_map3_def pw_algo_map2_def
+  apply refine_rcg
+              apply refine_dref_type
+              apply (simp; fail)+
+          apply (clarsimp, rule refine_aux; assumption)
+  by (auto intro: add_pw'_map3_ref pw_map_inv_ref)
+
+lemma pw_algo_map2_ref':
+  "pw_algo_map2 \<le> \<Down> (bool_rel \<times>\<^sub>r map_set_rel) pw_algo"
+proof -
+  note pw_algo_map2_ref
+  also note pw_algo_map_ref
+  also note pw_algo_unified_ref
+  finally show ?thesis .
+qed
+
+lemma pw_algo_map3_ref'[refine]:
+  "pw_algo_map3 \<le> \<Down> (bool_rel \<times>\<^sub>r (map_list_set_rel O map_set_rel)) pw_algo"
+proof -
+  have [simp]:
+    "((bool_rel \<times>\<^sub>r map_list_set_rel) O (bool_rel \<times>\<^sub>r map_set_rel))
+    = (bool_rel \<times>\<^sub>r (map_list_set_rel O map_set_rel))"
+    unfolding relcomp_def prod_rel_def by auto
+  note pw_algo_map3_ref
+  also note pw_algo_map2_ref'
+  finally show ?thesis
+    by (simp add: conc_fun_chain)
+qed
+
+end -- \<open>Worklist Map 2 Defs\<close>
+
+lemma (in Worklist_Map2_finite) map_set_rel_finite_domI[intro]:
+  "finite (dom m)" if "(m, S) \<in> map_set_rel"
+  using that unfolding map_set_rel_def by auto
+
+lemma (in Worklist_Map2_finite) map_set_rel_finiteI:
+  "finite S" if "(m, S) \<in> map_set_rel"
+  using that unfolding map_set_rel_def
+  apply clarsimp
+  apply (rule finite_Union)
+   apply (auto intro: map_dom_ran_finite; fail)
+  apply (auto simp: ran_def; fail)
+  done
+
+lemma (in Worklist_Map2_finite) map_set_rel_finite_ranI[intro]:
+  "finite S'" if "(m, S) \<in> map_set_rel" "S' \<in> ran m"
+  using that unfolding map_set_rel_def ran_def by auto
+
+locale Leadsto_Search_Space_Key =
+  A: Worklist_Map2 _ _ _ _ _ _ _ succs1 +
+  Leadsto_Search_Space
+  for succs1
+  (*
+  fixes key :: "'v \<Rightarrow> 'k"
+  assumes subsumes_key[intro, simp]: "a \<preceq> b \<Longrightarrow> key a = key b" *)
+begin
+
+sublocale A': Worklist_Map2_finite a\<^sub>0 "\<lambda> _. False" "op \<preceq>" empty "op \<unlhd>" E key succs1 "\<lambda> _. False"
+  by (standard; blast intro!: A.succs_correct)
+
+interpretation B:
+  Liveness_Search_Space_Key
+  "\<lambda> x y. E x y \<and> Q y \<and> \<not> empty y" a\<^sub>0 "\<lambda> _. False" "op \<preceq>" "\<lambda> x. A.reachable x \<and> \<not> empty x"
+  "\<lambda> _. False" succs key
+  apply standard
+    (* XXX This is not yet correct *)
+  sorry
+
+context
+  fixes a\<^sub>1 :: 'a
+begin
+
+interpretation B':
+  Liveness_Search_Space_Key
+  "\<lambda> x y. E x y \<and> Q y \<and> \<not> empty y" a\<^sub>1 "\<lambda> _. False" "op \<preceq>" "\<lambda> x. A.reachable x \<and> \<not> empty x"
+  "\<lambda> _. False" succs key
+  apply standard
+  subgoal
+    apply (subst succs_correct)
+    unfolding B.G.E'_def
+      apply auto
+    sorry
+  subgoal
+    by (rule A.finite_reachable)
+  subgoal
+    (* XXX This is not yet correct *)
+    sorry
+  done
+
+definition has_cycle_map where
+  "has_cycle_map = B'.dfs_map"
+
+lemmas has_cycle_map_ref[refine] = B'.dfs_map_dfs_refine[folded has_cycle_map_def has_cycle_def]
+
+end (* Second start state *)
+
+definition outer_inv where
+  "outer_inv passed done todo \<equiv> \<lambda> (r, passed').
+    (r \<longrightarrow> (\<exists> a. A.reachable a \<and> \<not> empty a \<and> P a \<and> Q a \<and> reaches_cycle a))
+     \<and> (\<not> r \<longrightarrow>
+          (\<forall> a \<in> \<Union> done. P a \<and> Q a \<longrightarrow> \<not> reaches_cycle a)
+         \<and> B.liveness_compatible passed'
+         \<and> passed' \<subseteq> {x. A.reachable x \<and> \<not> empty x}
+       )
+  "
+
+definition inner_inv where
+  "inner_inv passed done todo \<equiv> \<lambda> (r, passed').
+    (r \<longrightarrow> (\<exists> a. A.reachable a \<and> \<not> empty a \<and> P a \<and> Q a \<and> reaches_cycle a))
+     \<and> (\<not> r \<longrightarrow>
+          (\<forall> a \<in> done. P a \<and> Q a \<longrightarrow> \<not> reaches_cycle a)
+         \<and> B.liveness_compatible passed'
+         \<and> passed' \<subseteq> {x. A.reachable x \<and> \<not> empty x}
+       )
+  "
+
+definition leadsto' :: "bool nres" where
+  "leadsto' = do {
+    (r, passed) \<leftarrow> A'.pw_algo_map2;
+    let passed = ran passed;
+    (r, _) \<leftarrow> FOREACHcdi (outer_inv passed) passed (\<lambda>(b,_). \<not>b)
+      (\<lambda> passed' (_,acc).
+          FOREACHcdi (inner_inv acc) passed' (\<lambda>(b,_). \<not>b)
+            (\<lambda>v' (_,passed).
+              if P v' \<and> Q v' then has_cycle v' passed else RETURN (False, passed)
+            )
+            (False, acc)
+      )
+      (False, {});
+    RETURN r
+  }"
+
+lemma leadsto'_correct:
+  "leadsto' \<le> leadsto_spec"
+proof -
+  define inv where
+    "inv \<equiv> \<lambda> passed it (r, passed').
+       (r \<longrightarrow> (\<exists> a. A.reachable a \<and> \<not> empty a \<and> P a \<and> Q a \<and> reaches_cycle a))
+     \<and> (\<not> r \<longrightarrow>
+          (\<forall> a \<in> passed - it. \<not> reaches_cycle a)
+         \<and> B.liveness_compatible passed'
+         \<and> passed' \<subseteq> {x. A.reachable x \<and> \<not> empty x}
+       )
+    "
+
+  have [simp, intro]:
+    "\<not> A'.F_reachable"
+    unfolding A'.F_reachable_def by simp
+
+  have B_reaches_empty:
+    "\<not> empty b" if "\<not> empty a" "B.reaches a b" for a b
+    using that(2,1)by induction auto
+
+  interpret Subgraph_Start E a\<^sub>0 "\<lambda> a x. E a x \<and> Q x \<and> \<not> empty x"
+    by standard auto
+
+  have B_A_reaches:
+    "A.reaches a b" if "B.reaches a b" for a b
+    using that by (rule reaches)
+
+  have reaches_iff: "B.reaches a x \<longleftrightarrow> B.G.G'.reaches a x"
+    if "A.reachable a" "\<not> empty a" for a x
+    unfolding reaches_cycle_def thm B.G.E'_def
+    apply standard
+    using that
+      apply (rotate_tac 3)
+     apply (induction rule: rtranclp.induct)
+      apply blast
+     apply rule
+      apply assumption
+     apply (subst B.G.E'_def)
+    subgoal for a b c
+      by (auto dest: B_reaches_empty)
+    subgoal
+      by (rule B.G.reaches)
+    done
+
+  have reaches1_iff: "B.reaches1 a x \<longleftrightarrow> B.G.G'.reaches1 a x"
+    if "A.reachable a" "\<not> empty a" for a x
+    unfolding reaches_cycle_def
+    apply standard
+    subgoal
+      using that
+        apply (rotate_tac 3)
+      apply (induction rule: tranclp.induct)
+       apply (rule tranclp.intros(1), auto simp: B.G.E'_def; fail)
+      apply (
+          rule tranclp.intros(2);
+          auto 4 3 simp: B.G.E'_def dest:B_reaches_empty tranclp_into_rtranclp
+          )
+      done
+    subgoal
+      by (rule B.G.reaches1)
+    done
+
+  have reaches_cycle_iff: "reaches_cycle a \<longleftrightarrow> (\<exists>x. B.G.G'.reaches a x \<and> B.G.G'.reaches1 x x)"
+    if "A.reachable a" "\<not> empty a" for a
+    unfolding reaches_cycle_def
+    apply (subst reaches_iff[OF that])
+    using reaches1_iff B.G.G'_reaches_V that by blast
+
+  have aux1:
+    "\<not> reaches_cycle x"
+    if
+      "\<forall>a. A.reachable a \<and> \<not> empty a \<longrightarrow> (\<exists>x\<in>passed. a \<preceq> x)"
+      "passed \<subseteq> {a. A.reachable a \<and> \<not> empty a}"
+      "\<forall> y \<in> ran passed'. \<forall> x \<in> y. P x \<and> Q x \<longrightarrow> \<not> reaches_cycle x"
+      "A.reachable x" "\<not> empty x" "P x" "Q x"
+      "(passed', passed) \<in> A'.map_set_rel"
+    for x passed passed'
+  proof (rule ccontr, simp)
+    assume "reaches_cycle x"
+    from that obtain x' where x':"x' \<in> passed" "x \<preceq> x'"
+      by auto
+    with \<open>(_, _) \<in> _\<close> obtain y where y: "y \<in> ran passed'" "x' \<in> y"
+      unfolding A'.map_set_rel_def by auto
+    from x' that have "P x'" "Q x'"
+      by (auto intro: P_mono Q_mono)
+    with \<open>x' \<in> passed\<close> that(3) y have "\<not> reaches_cycle x'"
+      by auto
+    have "A.reachable x'" "\<not> empty x'"
+      using \<open>x' \<in> passed\<close> that(2) A.empty_mono \<open>x \<preceq> x'\<close> that(5) by auto
+    note reaches_cycle_iff' = reaches_cycle_iff[OF this] reaches_iff[OF this] reaches1_iff[OF this]
+    from \<open>reaches_cycle x\<close> guess y unfolding reaches_cycle_def
+      by safe
+    interpret
+      Subsumption_Graph_Pre_Nodes
+        "op \<preceq>" A.subsumes_strictly "\<lambda> x y. E x y \<and> Q y \<and> \<not> empty y" a\<^sub>0
+        "\<lambda> x. A.reachable x \<and> \<not> empty x"
+      by standard (rule B.mono[simplified]; assumption)
+    from \<open>B.reaches x y\<close> \<open>x \<preceq> x'\<close> \<open>B.reaches1 y y\<close> reaches_cycle_mono[OF B.finite_V] obtain y' where
+      "y \<preceq> y'" "B.G.G'.reaches x' y'" "B.G.G'.reaches1 y' y'"
+      apply atomize_elim
+      apply (subst (asm) reaches_iff[rotated 2])
+        defer
+        defer
+        apply (subst (asm) reaches1_iff)
+          defer
+          defer
+      using \<open>A.reachable x\<close> \<open>\<not> empty x\<close> \<open>A.reachable x'\<close> \<open>\<not> empty x'\<close> \<open>B.reaches1 y y\<close>
+      by (auto simp: B.reaches1_reaches_iff2 dest!: B.G.G'_reaches_V)
+    with \<open>A.reachable x'\<close> \<open>\<not> empty x'\<close> have "reaches_cycle x'"
+      unfolding reaches_cycle_iff'
+      by auto
+    with \<open>\<not> reaches_cycle x'\<close> show False ..
+  qed
+
+  note [refine_vcg] = A'.pw_algo_map2_correct[THEN order.trans]
+
+  show ?thesis
+    unfolding leadsto'_def leadsto_spec_def
+    apply (refine_rcg refine_vcg)
+
+      (* Input is finite 1 *)
+    subgoal
+      by (auto intro: map_dom_ran_finite)
+
+      (* Outer invariant holds initially *)
+      subgoal
+        unfolding outer_inv_def B.liveness_compatible_def by simp
+
+      (* Input is finite 2 *)
+      subgoal
+        by auto
+
+     (* Inner invariant holds initially *)
+      subgoal for x a b S1 S2 todo \<sigma> aa passed
+        unfolding inner_inv_def outer_inv_def by simp
+
+      subgoal for _ _ b S1 S2 xa \<sigma> aa passed S1' S2' a\<^sub>1 \<sigma>' ab passed'
+        unfolding outer_inv_def
+        apply clarsimp
+        subgoal premises prems for p
+        proof -
+            interpret B':
+              Liveness_Search_Space
+              "\<lambda> x y. E x y \<and> Q y \<and> \<not> empty y" a\<^sub>1 "\<lambda> _. False" "op \<preceq>"
+              "\<lambda> x. A.reachable x \<and> \<not> empty x" "\<lambda> _. False" succs
+              apply standard
+              subgoal
+                apply (subst succs_correct)
+                unfolding B.G.E'_def
+                 apply auto
+                sorry
+              subgoal
+                by (rule A.finite_reachable)
+              done
+            from prems have "a\<^sub>1 \<in> p"
+              unfolding A'.map_set_rel_def by auto
+            from \<open>inner_inv _ _ _ _\<close> have
+              "B'.liveness_compatible passed'" "passed' \<subseteq> {x. A.reachable x \<and> \<not> empty x}"
+              unfolding inner_inv_def by auto
+            from B'.dfs_correct[OF _ _ this] \<open>passed \<subseteq> _\<close> \<open>a\<^sub>1 \<in> _\<close> \<open>p \<subseteq> _\<close> have
+              "B'.dfs passed' \<le> B'.dfs_spec"
+              by auto
+            then show ?thesis
+              unfolding has_cycle_def
+              apply (rule order.trans)
+              unfolding B'.dfs_spec_def
+              apply clarsimp
+              subgoal for r passed1
+                apply (cases r)
+                 apply simp
+                subgoal
+                  unfolding inner_inv_def
+                  using \<open>passed \<subseteq> _\<close> \<open>a\<^sub>1 \<in> _\<close> \<open>p \<subseteq> _\<close>
+                  apply simp
+                  apply (inst_existentials a\<^sub>1)
+                  by (auto 4 3 simp: reaches_cycle_iff intro: prems)
+                subgoal
+                  using \<open>inner_inv _ _ _ _\<close> \<open>passed \<subseteq> _\<close> \<open>a\<^sub>1 \<in> _\<close> \<open>p \<subseteq> _\<close> reaches_cycle_iff
+                  unfolding inner_inv_def by auto
+                  done
+                done
+            qed
+            done
+
+          (* Current state filtered out *)
+          subgoal for x a b S1 S2 xa \<sigma> aa ba S1a S2a xb \<sigma>' ab bb
+            unfolding inner_inv_def by auto
+
+          (* Break \<and> inner inv \<longrightarrow> outer inv *)
+          subgoal for x a b S1 S2 xa \<sigma> aa ba S1a S2a \<sigma>'
+            unfolding inner_inv_def outer_inv_def by auto
+
+          (* \<not> Break \<and> inner inv \<longrightarrow> outer inv *)
+          subgoal for x a b S1 S2 xa \<sigma> aa ba \<sigma>'
+            unfolding inner_inv_def outer_inv_def by auto
+
+          (* Break \<and> outer inv \<longrightarrow> cycle *)
+          subgoal for x a b S1 S2 \<sigma> aa ba
+            unfolding outer_inv_def by auto
+
+          (* \<not> Break \<and> outer inv \<longrightarrow> cycle *)
+          (* I \<and> \<not> b \<longrightarrow> post *)
+          subgoal for x a b \<sigma> aa ba
+            unfolding outer_inv_def by (auto dest!: aux1)
+
+          done
+      qed
+
+lemma init_ref[refine]:
+  "((False, Map.empty), False, {}) \<in> bool_rel \<times>\<^sub>r A'.map_set_rel"
+  unfolding A'.map_set_rel_def by auto
+
+lemma map_set_rel_id:
+  "Liveness_Search_Space_Key.map_set_rel key = A'.map_set_rel"
+  unfolding A'.map_set_rel_def B.map_set_rel_def ..
+
+lemma has_cycle_map_ref'[refine]:
+  assumes "(P1, P1') \<in> A'.map_set_rel" "(a, a') \<in> Id"
+  shows "has_cycle_map a P1 \<le> \<Down> (bool_rel \<times>\<^sub>r A'.map_set_rel) (has_cycle a' P1')"
+  using has_cycle_map_ref assms by (auto simp: map_set_rel_id)
+
+definition leadsto_map3' :: "bool nres" where
+  "leadsto_map3' = do {
+    (r, passed) \<leftarrow> A'.pw_algo_map2;
+    let passed = ran passed;
+    (r, _) \<leftarrow> FOREACHcd passed (\<lambda>(b,_). \<not>b)
+      (\<lambda> passed' (_,acc).
+        do {
+          passed' \<leftarrow> SPEC (\<lambda>l. set l = passed');
+          nfoldli passed' (\<lambda>(b,_). \<not>b)
+            (\<lambda>v' (_,passed).
+              if P v' \<and> Q v' then has_cycle_map v' passed else RETURN (False, passed)
+            )
+            (False, acc)
+        }
+      )
+      (False, Map.empty);
+    RETURN r
+  }"
+
+definition "pw_algo_map2_copy = A'.pw_algo_map2"
+
+lemma [refine]:
+  "A'.pw_algo_map2 \<le>
+    \<Down> (br id (\<lambda> (_, m). finite (dom m) \<and> (\<forall> k S. m k = Some S \<longrightarrow> finite S))) pw_algo_map2_copy"
+proof -
+  have [refine]:
+    "(x, x') \<in> Id \<Longrightarrow>
+     x' = (x1, x2) \<Longrightarrow>
+     x = (x1a, x2a) \<Longrightarrow>
+     A'.pw_map_inv (x1, x2, False)
+    \<Longrightarrow> ((x1a, x2a, False), x1, x2, False) \<in>
+        (br id (\<lambda> m. finite (dom m) \<and> (\<forall> k S. m k = Some S \<longrightarrow> finite S))) \<times>\<^sub>r Id \<times>\<^sub>r Id"
+    for x x' x1 x2 x1a x2a
+    by (auto simp: br_def A'.pw_map_inv_def A'.map_set_rel_def)
+  show ?thesis
+    unfolding pw_algo_map2_copy_def
+    unfolding A'.pw_algo_map2_def
+    apply refine_rcg
+                  apply refine_dref_type
+                  prefer 5
+                  apply assumption
+                 apply (assumption | (simp add: br_def; fail) | (auto simp: br_def; fail))+
+    subgoal
+      apply (clarsimp simp: br_def)
+      subgoal premises prems
+        using \<open>finite _\<close> \<open>\<forall>k S. _ \<longrightarrow> finite _\<close>
+        unfolding A'.add_pw'_map2_def
+        apply refine_rcg
+           apply refine_dref_type
+           apply (auto simp: Let_def split!: option.split)
+        done
+      done
+    by (simp add: br_def)
+qed
+
+lemma leadsto_map3'_ref[refine]:
+  "leadsto_map3' \<le> \<Down> Id leadsto'"
+  unfolding leadsto_map3'_def leadsto'_def
+  apply (subst (2) pw_algo_map2_copy_def[symmetric])
+  apply (subst (2) FOREACHcdi_def)
+  apply (subst (2) FOREACHcd_def)
+  apply refine_rcg
+              apply refine_dref_type
+  by (auto simp: br_def intro: map_dom_ran_finite)
+
+definition leadsto_map3 :: "bool nres" where
+  "leadsto_map3 = do {
+    (r, passed) \<leftarrow> A'.pw_algo_map3;
+    let passed = ran passed;
+    (r, _) \<leftarrow> FOREACHcd passed (\<lambda>(b,_). \<not>b)
+      (\<lambda> passed' (_,acc).
+          nfoldli passed' (\<lambda>(b,_). \<not>b)
+            (\<lambda>v' (_,passed).
+              if P v' \<and> Q v' then has_cycle_map v' passed else RETURN (False, passed)
+            )
+            (False, acc)
+      )
+      (False, Map.empty);
+    RETURN r
+  }"
+
+lemma start_ref:
+  "((False, Map.empty), False, Map.empty) \<in> Id \<times>\<^sub>r map_list_set_rel"
+  by simp
+
+lemma map_list_set_rel_ran_set_rel:
+  "(ran ml, ran ms) \<in> \<langle>br set (\<lambda>_. True)\<rangle>set_rel" if "(ml, ms) \<in> map_list_set_rel"
+  using that unfolding map_list_set_rel_def set_rel_def
+  apply safe
+  subgoal for x
+    unfolding ran_def dom_def by force
+  subgoal for x'
+    unfolding ran_def by (auto dest!: A.map_list_set_relD[OF that] simp: br_def)
+  subgoal
+    unfolding Domain_fst br_def by auto
+  done
+
+lemma Id_list_rel_ref:
+  "(x'a, x'a) \<in> \<langle>Id\<rangle>list_rel"
+  by simp
+
+lemma map_list_set_rel_finite_ran:
+  "finite (ran ml)" if "(ml, ms) \<in> map_list_set_rel"
+  using that unfolding map_list_set_rel_def by (auto intro: map_dom_ran_finite)
+
+lemma leadsto_map3_ref[refine]:
+  "leadsto_map3 \<le> \<Down> Id leadsto'"
+  unfolding leadsto_map3_def leadsto'_def
+  apply (subst (2) FOREACHcdi_def)
+  apply (subst (2) FOREACHcd_def)
+  apply (refine_rcg map_list_set_rel_ran_set_rel map_list_set_rel_finite_ran)
+      prefer 4
+    apply (rule rhs_step_bind_SPEC)
+    apply (clarsimp simp: br_def; rule HOL.refl; fail)
+   apply (refine_rcg Id_list_rel_ref; simp; fail)
+   by auto
+
+definition leadsto_map4 :: "bool nres" where
+  "leadsto_map4 = do {
+    (r, passed) \<leftarrow> A'.pw_algo_map3;
+    ASSERT (finite (dom passed));
+    passed \<leftarrow> ran_of_map passed;
+    (r, _) \<leftarrow> nfoldli passed (\<lambda>(b,_). \<not>b)
+      (\<lambda> passed' (_,acc).
+          nfoldli passed' (\<lambda>(b,_). \<not>b)
+            (\<lambda>v' (_,passed).
+              if P v' \<and> Q v' then has_cycle_map v' passed else RETURN (False, passed)
+            )
+            (False, acc)
+      )
+      (False, Map.empty);
+    RETURN r
+  }"
+
+lemma ran_of_map_ref:
+  "ran_of_map m \<le> SPEC (\<lambda>c. (c, ran m') \<in> br set (\<lambda> _. True))" if "finite (dom m)" "(m, m') \<in> Id"
+  using ran_of_map_correct[OF that(1)] that(2) unfolding br_def by (simp add: pw_le_iff)
+
+lemma aux_ref:
+  "(xa, x'a) \<in> Id \<Longrightarrow>
+       x'a = (x1b, x2b) \<Longrightarrow> xa = (x1c, x2c) \<Longrightarrow> (x1c, x1b) \<in> bool_rel"
+  by simp
+
+definition "foo = A'.pw_algo_map3"
+
+lemma [refine]:
+  "A'.pw_algo_map3 \<le> \<Down> (br id (\<lambda> (_, m). finite (dom m))) foo"
+proof -
+  have [refine]:
+    "(x, x') \<in> Id \<Longrightarrow>
+     x' = (x1, x2) \<Longrightarrow>
+     x = (x1a, x2a) \<Longrightarrow>
+     A'.pw_map_inv3 (x1, x2, False)
+    \<Longrightarrow> ((x1a, x2a, False), x1, x2, False) \<in> (br id (\<lambda> m. finite (dom m))) \<times>\<^sub>r Id \<times>\<^sub>r Id"
+    for x x' x1 x2 x1a x2a
+    by (auto simp: br_def A'.pw_map_inv3_def map_list_set_rel_def)
+  show ?thesis
+    unfolding foo_def
+    unfolding A'.pw_algo_map3_def
+    apply refine_rcg
+                  apply refine_dref_type
+                  prefer 5
+                  apply assumption
+                 apply (assumption | (simp add: br_def; fail) | (auto simp: br_def; fail))+
+    subgoal
+      apply (clarsimp simp: br_def)
+      subgoal premises prems
+        using \<open>finite _\<close>
+        unfolding A'.add_pw'_map3_def
+        apply refine_rcg
+           apply refine_dref_type
+           apply (auto simp: Let_def)
+        done
+      done
+    by (simp add: br_def)
+qed
+
+lemma leadsto_map4_ref[refine]:
+  "leadsto_map4 \<le> \<Down> Id leadsto_map3"
+  unfolding leadsto_map4_def leadsto_map3_def FOREACHcd_def
+  apply (subst (2) foo_def[symmetric])
+  apply (refine_rcg ran_of_map_ref)
+     apply refine_dref_type
+     apply (simp add: br_def; fail)
+    apply (simp add: br_def; fail)
+   apply (rule rhs_step_bind_SPEC)
+  by (auto simp: br_def)
+
+definition leadsto_map4' :: "bool nres" where
+  "leadsto_map4' = do {
+    (r, passed) \<leftarrow> A'.pw_algo_map2;
+    ASSERT (finite (dom passed));
+    passed \<leftarrow> ran_of_map passed;
+    (r, _) \<leftarrow> nfoldli passed (\<lambda>(b,_). \<not>b)
+      (\<lambda> passed' (_,acc).
+        do {
+          passed' \<leftarrow> SPEC (\<lambda>l. set l = passed');
+          nfoldli passed' (\<lambda>(b,_). \<not>b)
+            (\<lambda>v' (_,passed).
+              if P v' \<and> Q v' then has_cycle_map v' passed else RETURN (False, passed)
+            )
+            (False, acc)
+        }
+      )
+      (False, Map.empty);
+    RETURN r
+  }"
+
+lemma leadsto_map4'_ref:
+  "leadsto_map4' \<le> \<Down> Id leadsto_map3'"
+  unfolding leadsto_map4'_def leadsto_map3'_def FOREACHcd_def
+  apply (subst (2) pw_algo_map2_copy_def[symmetric])
+  apply (refine_rcg ran_of_map_ref)
+     apply refine_dref_type
+     apply (simp add: br_def; fail)
+    apply (simp add: br_def; fail)
+   apply (rule rhs_step_bind_SPEC)
+  by (auto simp: br_def)
+
+lemma leadsto_map4'_correct:
+  "leadsto_map4' \<le> leadsto_spec_alt"
+proof -
+  note leadsto_map4'_ref
+  also note leadsto_map3'_ref
+  also note leadsto'_correct
+  also note leadsto_spec_leadsto_spec_alt
+  finally show ?thesis .
+qed
+
+end (* Leadsto Search Space Key *)
+
+end (* Theory *)
