Worklist_Algorithms/Next_Key.thy
@@ -1,0 +1,219 @@
+theory Next_Key
+  imports Heap_Hash_Map
+begin
+
+section \<open>A next-key operation for hashmaps\<close>
+
+subsection \<open>Definition and key properties\<close>
+
+definition
+  "hm_it_next_key ht = do {
+    n\<leftarrow>Array.len (the_array ht);
+    if n = 0 then raise ''Map is empty!''
+    else do {
+      i\<leftarrow>hm_it_adjust (n - 1) ht;
+      l\<leftarrow>Array.nth (the_array ht) i;
+      case l of
+        [] \<Rightarrow> raise ''Map is empty!''
+      | (x # _) \<Rightarrow> return (fst x)
+    }
+  }
+"
+
+lemma hm_it_next_key_rule:
+  "<is_hashmap m ht> hm_it_next_key ht <\<lambda>r. is_hashmap m ht * \<up> (r \<in> dom m)>"
+  if "m \<noteq> Map.empty"
+  using that
+  unfolding hm_it_next_key_def
+  unfolding is_hashmap_def unfolding is_hashmap'_def
+  apply (sep_auto intro: hm_it_adjust_rule)
+  subgoal
+    using le_imp_less_Suc by fastforce
+  subgoal premises prems for l xs i xs'
+  proof -
+    from prems have "l ! i \<noteq> []"
+      by (auto simp: concat_take_Suc_empty)
+    with prems(1-6) show ?thesis
+      apply (cases xs')
+       apply sep_auto
+      apply sep_auto
+      subgoal for a b list aa ba
+        apply (rule weak_map_of_SomeI[of _ b])
+        apply auto
+        apply (rule bexI[of _ "l ! i"])
+        subgoal
+          by (metis list.set_intros(1))
+        subgoal
+          by (cases "length l"; fastforce simp: take_Suc_conv_app_nth)
+        done
+      done
+  qed
+  done
+
+lemma
+  "<P * R> c <\<lambda> r. Q r * R>" if "<P> c <\<lambda> r. Q r>"
+  using that
+  by (simp add: frame_rule)
+
+
+definition
+  "next_key m = do {
+    ASSERT (m \<noteq> Map.empty);
+    k \<leftarrow> SPEC (\<lambda> k. k \<in> dom m);
+    RETURN k
+  }
+  "
+
+lemma hm_it_next_key_next_key_aux:
+  fixes K :: "_ :: {hashable, heap} \<Rightarrow> _"
+  assumes "CONSTRAINT is_pure K" "nofail (next_key m)"
+  shows
+    "<hm.assn K V m mi>
+      hm_it_next_key mi
+    <\<lambda>r. \<exists>\<^sub>Axa. hm.assn K V m mi * K xa r * true * \<up> (RETURN xa \<le> next_key m)>"
+  using \<open>nofail _\<close> unfolding next_key_def
+  apply (simp add: pw_bind_nofail pw_ASSERT(1))
+  unfolding hm.assn_def hr_comp_def
+  apply sep_auto
+  subgoal for m'
+    apply (rule cons_post_rule)
+     apply (rule hm_it_next_key_rule)
+     defer
+     apply (sep_auto eintros del: exI)
+    subgoal premises prems for x v'
+    proof -
+      from prems obtain k v where "m k = Some v" "(x, k) \<in> the_pure K" "(v', v) \<in> the_pure V"
+        apply atomize_elim
+        by (meson map_rel_obtain2)
+      with prems \<open>CONSTRAINT is_pure K\<close> show ?thesis
+        apply -
+        apply (rule exI[where x = k], rule exI[where x = m'])
+        apply sep_auto
+        apply (rule entailsI)
+        apply sep_auto
+        by (metis mod_pure_star_dist mod_star_trueI pure_def pure_the_pure)
+    qed
+    by force
+  done
+
+lemma hm_it_next_key_next_key:
+  fixes K :: "_ :: {hashable, heap} \<Rightarrow> _"
+  assumes "CONSTRAINT is_pure K"
+  shows
+    "(hm_it_next_key, next_key) \<in> (hm.assn K V)\<^sup>k \<rightarrow>\<^sub>a K"
+  using assms by sepref_to_hoare (sep_auto intro!: hm_it_next_key_next_key_aux)
+
+lemma hm_it_next_key_next_key':
+  shows
+    "(hm_it_next_key, next_key) \<in> (hm.hms_assn V)\<^sup>k \<rightarrow>\<^sub>a id_assn"
+  unfolding hm.hms_assn_def
+  apply sepref_to_hoare
+  apply sep_auto
+  unfolding next_key_def
+  apply (simp add: refine_pw_simps)
+  subgoal for m m' mi
+    apply (rule cons_rule[where
+          P' = "is_hashmap mi m' * map_assn V m mi * \<up>(mi \<noteq> Map.empty)"
+          and Q = "\<lambda> x. is_hashmap mi m' * \<up> (x \<in> dom mi) * map_assn V m mi"]
+        )
+      apply (sep_auto; unfold map_assn_def; auto; fail)+
+    apply (rule norm_pre_pure_rule1)
+    apply (rule frame_rule[OF hm_it_next_key_rule[of mi m']])
+    by (sep_auto; unfold map_assn_def; auto)+
+  done
+
+subsection \<open>Computing the range of a map\<close>
+
+definition ran_of_map where
+  "ran_of_map m \<equiv> do
+      {
+        (xs, m) \<leftarrow> WHILEIT
+          (\<lambda> (xs, m'). finite (dom m') \<and> ran m = ran m' \<union> set xs) (\<lambda> (_, m). Map.empty \<noteq> m)
+            (\<lambda> (xs, m). do
+              {
+                k \<leftarrow> next_key m;
+                let (x, m) = op_map_extract k m;
+                ASSERT (x \<noteq> None);
+                RETURN (the x # xs, m)
+              }
+            )
+            ([], m);
+        RETURN xs
+      }
+  "
+
+context
+begin
+
+private definition
+  "ran_of_map_var = (inv_image (measure (card o dom)) (\<lambda> (a, b). b))"
+
+private lemma wf_ran_of_map_var:
+  "wf ran_of_map_var"
+  unfolding ran_of_map_var_def by auto
+
+(* XXX Maybe move *)
+private lemma insert_restrict_ran:
+  "insert v (ran (m |` (- {k}))) = ran m " if "m k = Some v"
+  using that unfolding ran_def restrict_map_def by force
+
+lemma ran_of_map_correct[refine]:
+  "ran_of_map m \<le> SPEC (\<lambda> r. set r = ran m)" if "finite (dom m)"
+  using that unfolding ran_of_map_def next_key_def
+  apply (refine_vcg wf_ran_of_map_var)
+         apply (simp; fail)
+        apply (simp; fail)
+       apply (simp; fail)
+      apply (clarsimp; fail)
+     apply (clarsimp; fail)
+  subgoal
+    unfolding dom_def by (clarsimp, auto dest: insert_restrict_ran)
+  subgoal
+    unfolding ran_of_map_var_def op_map_extract_def by (fastforce intro: card_Diff1_less)
+  by auto
+
+end -- \<open>End of private context for auxiliary facts and definitions\<close>
+
+sepref_register next_key :: "(('b, 'a) i_map \<Rightarrow> 'b nres)"
+
+definition (in imp_map_is_empty) [code_unfold]: "hms_is_empty \<equiv> is_empty"
+
+lemma (in imp_map_is_empty) hms_empty_rule [sep_heap_rules]:
+  "<hms_assn A m mi> hms_is_empty mi <\<lambda>r. hms_assn A m mi * \<up>(r \<longleftrightarrow> m=Map.empty)>\<^sub>t"
+  unfolding hms_is_empty_def hms_assn_def map_assn_def by sep_auto
+
+context imp_map_is_empty
+begin
+
+lemma hms_is_empty_hnr[sepref_fr_rules]:
+  "(hms_is_empty, RETURN o op_map_is_empty) \<in> (hms_assn A)\<^sup>k \<rightarrow>\<^sub>a bool_assn"
+  by sepref_to_hoare sep_auto
+
+sepref_decl_impl is_empty: hms_is_empty_hnr uses op_map_is_empty.fref[where V = Id] .
+print_theorems
+
+end
+
+lemma (in imp_map) hms_assn'_id_hms_assn:
+  "hms_assn' id_assn A = hms_assn A"
+  by (subst hms_assn'_def) simp
+
+(* This is to make the pre-processing phase pick the right type for the input *)
+lemma [intf_of_assn]:
+  "intf_of_assn (hm.hms_assn' a b) TYPE(('aa, 'bb) i_map)"
+  by simp
+
+context
+  notes [sepref_fr_rules] = hm_it_next_key_next_key'[folded hm.hms_assn'_id_hms_assn]
+begin
+
+sepref_definition ran_of_map_impl is
+  "ran_of_map" :: "(hm.hms_assn A)\<^sup>d \<rightarrow>\<^sub>a list_assn A"
+  unfolding ran_of_map_def hm.hms_assn'_id_hms_assn[symmetric]
+  unfolding op_map_is_empty_def[symmetric]
+  unfolding hm.hms_fold_custom_empty HOL_list.fold_custom_empty
+  by sepref
+
+end (* End of anonymous context for setup *)
+
+end (* Theory *)
